renamed random generators

Azurite/Random/Bool.lean
@@ -8,17 +8,17 @@ namespace Azurite.Random
 A generic generator modifier that takes a `UInt64` generator and yields `Bool`s efficiently,
 stretching a single `UInt64` into 64 boolean values.
 -/
-structure BoolGen (G : Type) [RandomGen G UInt64] where
+structure BoolRandomGen (G : Type) [RandomGen G UInt64] where
   gen : G
   cache : UInt64
   bitsLeft : Nat
   deriving Repr
 
 /-- Initialize the efficient `Bool` generator spanning from an underlying `UInt64` PRNG. -/
-def mkBoolGen (seed : UInt64) : BoolGen SplitMix64 :=
+def mkBoolRandomGen (seed : UInt64) : BoolRandomGen SplitMix64 :=
   { gen := mkSplitMix64 seed, cache := 0, bitsLeft := 0 }
 
-def BoolGen.next {G : Type} [RandomGen G UInt64] (bg : BoolGen G) : Bool × BoolGen G :=
+def BoolRandomGen.next {G : Type} [RandomGen G UInt64] (bg : BoolRandomGen G) : Bool × BoolRandomGen G :=
   if bg.bitsLeft == 0 then
     let (newCache, newGen) : UInt64 × G := RandomGen.next bg.gen
     let b := (newCache &&& (1 : UInt64)) == (1 : UInt64)
@@ -29,22 +29,22 @@ def BoolGen.next {G : Type} [RandomGen G UInt64] (bg : BoolGen G) : Bool × Bool
     let nextBg := { bg with cache := bg.cache >>> (1 : UInt64), bitsLeft := bg.bitsLeft - 1 }
     (b, nextBg)
 
-instance {G : Type} [RandomGen G UInt64] : RandomGen (BoolGen G) Bool where
-  next := BoolGen.next
+instance {G : Type} [RandomGen G UInt64] : RandomGen (BoolRandomGen G) Bool where
+  next := BoolRandomGen.next
 
 /--
 A generator that produces `Bool`s where `true` is weighted by a given rational probability `0 < p < 1`.
 -/
-structure WeightedBoolGen (G : Type) [RandomGen G UInt64] where
-  natGen : NatLessThanGen G
+structure WeightedBoolRandomGen (G : Type) [RandomGen G UInt64] where
+  natGen : NatLessThanRandomGen G
   p : Rat
   deriving Repr
 
-/-- Initialize the `WeightedBoolGen` given a rational probability `p = n / d`. -/
-def mkWeightedBoolGen (p : Rat) (seed : UInt64) : WeightedBoolGen SplitMix64 :=
-  { natGen := mkNatLessThanGen p.den seed, p := p }
+/-- Initialize the `WeightedBoolRandomGen` given a rational probability `p = n / d`. -/
+def mkWeightedBoolRandomGen (p : Rat) (seed : UInt64) : WeightedBoolRandomGen SplitMix64 :=
+  { natGen := mkNatLessThanRandomGen p.den seed, p := p }
 
-def WeightedBoolGen.next {G : Type} [RandomGen G UInt64] (bg : WeightedBoolGen G) : Bool × WeightedBoolGen G :=
+def WeightedBoolRandomGen.next {G : Type} [RandomGen G UInt64] (bg : WeightedBoolRandomGen G) : Bool × WeightedBoolRandomGen G :=
   if bg.p ≤ 0 then
     (false, bg)
   else if 1 ≤ bg.p then
@@ -54,7 +54,7 @@ def WeightedBoolGen.next {G : Type} [RandomGen G UInt64] (bg : WeightedBoolGen G
     let b := val < bg.p.num.toNat
     (b, { bg with natGen := nextNatGen })
 
-instance {G : Type} [RandomGen G UInt64] : RandomGen (WeightedBoolGen G) Bool where
-  next := WeightedBoolGen.next
+instance {G : Type} [RandomGen G UInt64] : RandomGen (WeightedBoolRandomGen G) Bool where
+  next := WeightedBoolRandomGen.next
 
 end Azurite.Random
